\documentclass[]{article}
\usepackage{amsmath}
\usepackage{amssymb}
\usepackage[margin=0.5in]{geometry}
\usepackage{hyperref}

%opening
\title{The Gradient}
\author{Benjamin S. Knight}

\begin{document}
\maketitle
\begin{equation} \label{eq1}
\begin{split}
\displaystyle\frac{\delta E}{\delta y} & = \displaystyle\frac{\delta}{\delta y}\Big(1/2\sum(y^\mu - \hat{y}^\mu)^2\Big)\\
& = 2(1/2)\sum(y^\mu - \hat{y}^\mu)^1\\
& = \sum(y^\mu - \hat{y}^\mu) \text{\phantom{aaaa}} \rightarrow \text{\phantom{aaaa}} y^\mu - \hat{y}^\mu \\
& \text{\phantom{aaaaaaaaaaaaaaaaaaaaaaaaaaa}} \big\downarrow\\
& \text{\phantom{aaaaaaaaaaaaaaaaaaaaaaaaa}} 1 - 0.21\\
& \text{\phantom{aaaaaaaaaaaaaaaaaaaaaaaaaaa}} \big\downarrow\\
& \text{\phantom{aaaaaaaaaaaaaaaaaaaaaaaaaa}} 0.79
\end{split}
\end{equation}

\begin{equation} \label{eq1}
\begin{split}
\displaystyle\frac{\delta}{\delta x}\sigma(x) & = \sigma(x)(1 - \sigma(x))\\
 & \text{\phantom{aaaaaaaa}} \big\downarrow \\
\displaystyle\frac{\delta E}{\delta \sigma} & = (y - \hat{y})\sigma(x)(1 - \sigma(x))\\
& = (1 - 0.21)\Big(\displaystyle\frac{1}{1 + e^{-(-1.28)}}\Big)\Big(1 - \displaystyle\frac{1}{1 + e^{-(-1.28)}}\Big)\\
& = (1 - 0.21)(0.21)(1 - 0.21)\\
& = (0.79)(0.21)(0.79)\\
& = 0.131\\
\end{split}
\end{equation}




\begin{equation} \label{eq1}
\begin{split}
f(o1) & = h_1(W_{h1}^{o1}) + h_2(W_{h2}^{o1}) \text{\phantom{aaa}} \rightarrow \text{\phantom{aaa}} \displaystyle\frac{\partial o_1}{\partial h_1} = W_{h1}^{o1} = 0.7  \\
& \text{\phantom{||||aaaaaaaaaaaaaaaaaaaaaaaaaaaaa}} \displaystyle\frac{\partial o_1}{\partial h_2} = W_{h2}^{o1} = -0.6
\end{split}
\end{equation}

\begin{equation} \label{eq1}
\begin{split}
f(h1) & = x_1(W_{x1}^{h1}) + x_2(W_{x2}^{h1}) \text{\phantom{aaa}} \rightarrow \text{\phantom{aaa}} \displaystyle\frac{\partial h_1}{\partial x_1} = W_{x1}^{h1} = 0.3 \\
& \text{\phantom{||||aaaaaaaaaaaaaaaaaaaaaaaaaaaaa}} \displaystyle\frac{\partial h_1}{\partial x_2} = W_{x2}^{h1} = 0.8
\end{split}
\end{equation}

\begin{equation} \label{eq1}
\begin{split}
f(h2) & = x_1(W_{x1}^{h2}) + x_2(W_{x2}^{h2}) \text{\phantom{aaa}} \rightarrow \text{\phantom{aaa}} \displaystyle\frac{\partial h_2}{\partial x_1} = W_{x1}^{h2} = -0.1 \\
& \text{\phantom{||||aaaaaaaaaaaaaaaaaaaaaaaaaaaaa}} \displaystyle\frac{\partial h_2}{\partial x_2} = W_{x2}^{h2} = -0.5
\end{split}
\end{equation}

Weight recalculations:
\begin{equation} \label{eq1}
\begin{split}
f(h2) & = x_1(W_{x1}^{h2}) + x_2(W_{x2}^{h2}) \text{\phantom{aaa}} \rightarrow \text{\phantom{aaa}} \displaystyle\frac{\partial h_2}{\partial x_1} = W_{x1}^{h2} = -0.1 \\
& \text{\phantom{||||aaaaaaaaaaaaaaaaaaaaaaaaaaaaa}} \displaystyle\frac{\partial h_2}{\partial x_2} = W_{x2}^{h2} = -0.5
\end{split}
\end{equation}


\[ 1/2 \sum(y^\mu - \hat{y}^\mu)^2 \]

\[ y^\mu - \hat{y}^\mu \]

\[ \sigma(x) \]

\[ \sigma(x)(1 - \sigma(x)) \]

\[ h_1(W_{h1}^{o1}) + h_2(W_{h2}^{o1}) \rightarrow  \displaystyle\frac{\partial o_1}{\partial h_1}\]


\end{document}